WIP

theories/types/UniverseLevel.v
@@ -1,4 +1,4 @@
-Require Import Overture.
+Require Import Overture types.Universe PathGroupoids Equivalences EquivalenceVarieties types.Paths.
 
 Set Implicit Arguments.
 
@@ -6,19 +6,9 @@ Set Implicit Arguments.
 
 (** We provide casting definitions for raising universe levels. *)
 
-Section local.
-  Let type_cast_up_type : Type.
-  Proof.
-    let U0 := constr:(Type) in
-    let U1 := constr:(Type) in
-    let unif := constr:(U0 : U1) in
-    exact (U0 -> U1).
-  Defined.
-
-  (** Because we have cumulativity (that [T : Uᵢ] gives us [T : Uᵢ₊₁]), we may define [Lift : U₀ → U₁] as the identity function with a fancy type; the type says that [U₀ ⊊ U₁]. *)
-  Definition Lift : type_cast_up_type
-    := fun T => T.
-End local.
+(** Because we have cumulativity (that [T : Uᵢ] gives us [T : Uᵢ₊₁]), we may define [Lift : U₀ → U₁] as the identity function with a fancy type; the type says that [U₀ ⊊ U₁]. *)
+Definition Lift : Type@{i} -> Type@{j}
+  := Eval hnf in let lt := Type@{i} : Type@{j} in fun T => T.
 
 Definition lift {T} : T -> Lift T := fun x => x.
 Global Instance isequiv_lift T : IsEquiv (@lift T)
@@ -33,6 +23,138 @@ Definition lower {A} := (@equiv_inv _ _ (@lift A) _).
 
 (** We make [lift] and [lower] opaque so that typeclass resolution doesn't pick up [isequiv_lift] as an instance of [IsEquiv idmap] and wreck havok. *)
 Typeclasses Opaque lift lower.
+
+Instance isembedding_Lift `{Univalence} x y : IsEquiv (@ap _ _ Lift x y).
+Proof.
+  refine (isequiv_adjointify _ _ _ _).
+  { intro H'.
+    pose proof ((fun H0 => (@path_universe _ _ _ (@lift x) (H0 x) @ H' @ (@path_universe _ _ _ (@lift y) (H0 y))^)))%path as H''.
+    set (id := fun T (x : T) => x).
+    change @IsEquiv with (id _ (@IsEquiv)) in *.
+    refine (match H'' _ with idpath => idpath end).
+    subst id; simpl.
+    intro.
+    exact (@BuildIsEquiv
+             _ _
+             (fun x => x)
+             (fun x => x)
+             (fun _ => idpath)
+             (fun _ => idpath)
+             (fun _ => idpath)). }
+  { hnf; simpl.
+    intro x0.
+    revert x0.
+    intro x0.
+    pattern x0.
+    rewrite <- !(eta_path_universe x0).
+    SearchAbout path_universe.
+    Set Printing Implicit.
+
+    match goal with
+    unfold Lift, lower, lift in H''; simpl in H''.
+    apply H''.
+
+
+
+intro H'; apply path_universe_uncurried; apply equiv_path in H'.
+    refine (BuildEquiv _ _ _ (BuildIsEquiv _ _ _ _ _ _ _)).
+    { exact (lower o equiv_fun H' o lift). }
+    { exact (lower o @equiv_inv _ _ _ H' o lift). }
+    { intro H''.
+      change ((lower o H' o H'^-1%equiv o lift) H'' = H'').
+      exact (ap lower (eisretr H' (lift H''))). }
+    { intro H''.
+      change ((lower o H'^-1%equiv o H' o lift) H'' = H'').
+      exact (ap lower (eissect H' (lift H''))). }
+    { intro x0; cbv beta.
+
+      lazymatch goal with
+      | [ |- ?a = ?b :> ?T ]
+        => pose (a:T)
+      end.
+
+      refine (_ @ (ap_compose (H' o lift) lower (ap lower (eissect H' (lift x0))))^)%path.
+      refine (_ @ (ap_compose lower (lower o H' o lift) (eissect H' (lift x0))))%path.
+      refine (
+      apply (@equiv_inv _ _ (ap (ap lift)) (isequiv_ap _ _)).
+      refine ((ap_compose lower lift _)^ @ _)%path.
+      change (@lift ?T o lower) with (fun x : T => x).
+      refine (ap_idmap _ @ _)%path.
+      refine (eisadj H' x0 @ _)%path.
+      apply (@equiv_inv _ _ (ap (ap lower)) (@isequiv_ap _ _ _ (@isequiv_ap _ _ _ (isequiv_inverse) _ _) _ _)).
+      refine (_ @ (ap_compose lift lower _))%path.
+      change (@lower ?T o lift) with (fun x : T => x).
+      refine (_ @ (ap_idmap _)^)%path.
+      apply (@equiv_inv _ _ (ap (ap H'%equiv)) (@isequiv_ap _ _ _ (@isequiv_ap _ _ _ (isequiv_inverse) _ _) _ _)).
+      refine (_ @ (ap_compose lower H' _))%path.
+
+      SearchAbout ap.
+      apply (ap lift)^-1%equiv.
+
+      exact idpath.
+      Set Printing All.
+      Set Printing Universes.
+      apply H''''.
+      apply H''''.
+      simpl in *.
+      pose (fun X => (H'''' X)) as H'''''.
+
+
+      SearchAbout Equiv paths.
+      speci
+
+    { intro.
+      let p := constr:((transport_pp idmap H'^ H' x0)^)%path in
+      lazymatch type of p with
+      | ?a = ?b :> ?T
+        => refine (match p in (_ = y) return (a = y) with 1 => 1 end @ _)%path
+      end.
+      pattern (H'^ @ H')%path.
+      refine (transport _ (@concat_Vp _ _ _ H')^%path idpath). }
+    { intro.
+      let p := constr:((transport_pp idmap H' H'^ x0)^)%path in
+      lazymatch type of p with
+      | ?a = ?b :> ?T
+        => refine (match p in (_ = y) return (a = y) with 1 => 1 end @ _)%path
+      end.
+      pattern (H' @ H'^)%path.
+      refine (transport _ (@concat_pV _ _ _ H')^%path idpath). } }
+  { intro H'; simpl.
+
+    SearchAbout path_universe.
+    refine (ap_idmap _ @ _)%path.
+    SearchAbout (ap idmap _).
+
+    rewrite transport_idmap_ap.
+
+
+      { exact idpath. }
+      { pose .
+      { by destruct H'. }
+      rewrite <- transport_pp
+      rewrite concat_Vp.
+      simpl.
+      reflexivity.
+      SearchAbout transport.
+
+      Set Printing All.
+      Set Printing Universes.
+
+
+SearchAbout transport inverse.
+    refine (match H' in (_ = y') return (x <~> y)%equiv ->  with
+              | idpath => _
+            end).
+induction H'.
+
+  Set Printing All. Set Printing Universes.
+
+
+
+Set Printing Universes.
+
+
+
 
 
 (*Fail Check Lift nat : Type0.
